propositional, need to add total variable count

theories/Logic/definitions.v
@@ -18,6 +18,4 @@ Lemma or_bool_prop : forall (b1 b2 : bool),
   b1 || b2 = true -> b1 = true \/ b2 = true.
 Proof. intros. case_eq b1; case_eq b2; intros; rewrite H0,H1 in H; auto. Qed.
 
-Definition ivar := nat.
-
 Definition ovar := nat.
