theories/Logic/fol.v
@@ -21,29 +21,22 @@ Open Scope list_scope.
 Import ListNotations.
 
 (*Language*)
-Inductive nvec : nat -> Type :=
-| Null : nvec 0
-| New : forall {m : nat}, nat -> nvec m -> nvec (S m).
 
-Inductive predicate : nat -> Type :=
-| Nullary : forall (i : nat), predicate 0
-| Succary : forall {m : nat} (i : nat) (prd : predicate m), @predicate (S m)
-| Var : forall {n : nat} (i : nat), predicate n.
+Inductive predicate : Type :=
+| Nullary : forall (i : nat), predicate
+| Var : forall (i : nat), predicate.
 
-Fixpoint pure_predicate {n : nat} (pn : predicate n) : bool :=
+Definition pure_predicate (pn : predicate) : bool :=
 match pn with
 | Nullary _ => true
-| Succary _ pn' => pure_predicate pn'
 | Var _ => false
 end.
 
 Inductive formula : Type :=
 | fal : formula
-| equ : ivar -> ivar -> formula
 | imp : formula -> formula -> formula
-| univ : formula -> formula
 | bnd : ovar -> ovar -> formula -> formula
-| prd : forall {n : nat} (vec : nvec n) (pn : predicate n), pure_predicate pn = true -> formula.
+| prd : forall (pn : predicate), pure_predicate pn = true -> formula.
 (*
 | mu : forall n, (predicate n) -> formula -> formula
 | muk : forall n, (predicate n) -> ordinal -> formula -> formula.
@@ -52,565 +45,83 @@ Inductive formula : Type :=
 Fixpoint num_conn (A : formula) : ordinal :=
 match A with
 | fal => cast Zero
-| equ v1 v2 => cast Zero
 | imp B C => oadd (oadd (num_conn B) (num_conn C)) (cast (nat_ord 1))
-| univ B => oadd (num_conn B) (cast (nat_ord 1))
 | bnd o1 o2 B => oadd (num_conn B) (cast (nat_ord 1))
-| prd vec pn pure => cast Zero
+| prd pn pure => cast Zero
 end.
 
 Fixpoint vars_in (a : formula) : list ovar :=
 match a with
 | fal => []
-| equ v1 v2 => []
 | imp B C => (vars_in B) ++ (vars_in C)
-| univ B => (vars_in B)
 | bnd o1 o2 B => o2 :: remove nat_eq_dec o1 (vars_in B)
-| prd vec pn pure => []
+| prd pn pure => []
 end.
 
-Fixpoint nvec_eqb {n1 n2 : nat} (vec1 : nvec n1) (vec2 : nvec n2) : bool :=
-match vec1, vec2 with
-| Null, Null => true (*nat_eqb m1 m2*)
-| New m1 vec1', New m2 vec2' => nat_eqb m1 m2 && nvec_eqb vec1' vec2'
+Definition prd_eqb (pn1 pn2 : predicate) : bool :=
+match pn1, pn2 with
+| Nullary i1, Nullary i2 => nat_eqb i1 i2
+| Var i1, Var i2 => nat_eqb i1 i2
 | _, _ => false
-end.
-
-Fixpoint prd_eqb {n1 n2 : nat} (pn1 : predicate n1) (pn2 : predicate n2) : bool :=
-match nat_eqb n1 n2 with
-| true => match pn1, pn2 with
-    | Nullary i1, Nullary i2 => nat_eqb i1 i2
-    | Succary i1 pn1', Succary i2 pn2'  => nat_eqb i1 i2 && prd_eqb pn1' pn2'
-    | Var i1, Var i2 => nat_eqb i1 i2
-    | _ , _ => false
-    end
-| false => false
 end.
 
 Fixpoint form_eqb (A1 A2 : formula) : bool :=
 match A1, A2 with
 | fal, fal => true
-| equ v1 v2, equ v3 v4 => nat_eqb v1 v3 && nat_eqb v2 v4
 | imp B1 C1, imp B2 C2 => form_eqb B1 B2 && form_eqb C1 C2
-| univ B1, univ B2 => form_eqb B1 B2
 | bnd o1 o2 B1, bnd o3 o4 B2 => nat_eqb o1 o3 && nat_eqb o2 o4 && form_eqb B1 B2
-| prd vec1 pn1 _, prd vec2 pn2 _ => nvec_eqb vec1 vec2 && prd_eqb pn1 pn2
+| prd pn1 _, prd pn2 _ => prd_eqb pn1 pn2
 | _, _ => false
 end.
-
-(*
-Fixpoint in_vecb {n : nat} (vec : nvec n) (i : ivar) : bool :=
-match vec with
-| Null => false
-| New v vec' => nat_eqb v i || in_vecb vec' i
-end.
-
-Fixpoint free_var (phi : formula) (i : ivar) : bool :=
-match phi with
-| fal => false
-| equ v1 v2 => nat_eqb v1 i || nat_eqb v2 i
-| imp B C => free_var B i || free_var C i
-| univ B => match i with
-    | 0 => false
-    | S n => free_var B n
-    end
-| bnd o1 o2 B => free_var B i
-| prd vec pn pure => in_vecb vec i
-end.
-*)
 
 Fixpoint form_depth (phi : formula) : nat :=
 match phi with
 | fal => 0
-| equ v1 v2 => 0
 | imp B C => max (form_depth B) (form_depth C)
-| univ B => S (form_depth B)
 | bnd o1 o2 B => form_depth B
-| prd vec pn pure => 0
+| prd pn pure => 0
 end.
-
-Fixpoint vec_map {n : nat} (F : nat -> nat) (vec : nvec n) : nvec n :=
-match vec with
-| Null => Null
-| New v vec' => New (F v) (vec_map F vec')
-end.
-
-(*
-Fixpoint shift_subst (A : formula) (i1 i2 : ivar) : formula :=
-match A with
-| fal => fal
-| equ v1 v2 =>
-    match nat_semiconnex_type v1 i1, nat_semiconnex_type v2 i1 with
-    | inl (inl GT1), inl (inl GT2) => equ (pred v1) (pred v2)
-    | inl (inl GT1), inl (inr EQ2) => equ (pred v1) (v2 + i2)
-    | inl (inl GT1), inr LT2 => equ (pred v1) v2
-    | inl (inr EQ1), inl (inl GT2) => equ (v1 + i2) (pred v2)
-    | inl (inr EQ1), inl (inr EQ2) => equ (v1 + i2) (v2 + i2)
-    | inl (inr EQ1), inr LT2 => equ (v1 + i2) v2
-    | inr LT1, inl (inl GT2) => equ v1 (pred v2)
-    | inr LT1, inl (inr EQ2) => equ v1 (v2 + i2)
-    | inr LT1, inr LT2 => equ v1 v2
-    end
-| imp B C => imp (shift_subst B i1 i2) (shift_subst C i1 i2) 
-| univ B => univ (shift_subst B (S i1) i2)
-| bnd o1 o2 B => bnd o1 o2 (shift_subst B i1 i2)
-| prd vec pn pure =>
-    prd
-    (vec_map (fun n => match nat_semiconnex_type n i1 with
-              | inl (inl GT) => (pred n)
-              | inl (inr EQ) => (n + i2)
-              | inr LT => n
-              end) vec)
-    pn pure
-end.
-
-Lemma shift_subst_lemma :
-    forall (phi : formula) (i1 j1 i2 i3 : ivar),
-        shift_subst (shift_subst A i1 i2) (i1 + j1) i3 = shift_subst (shift_subst A (S (i1 + j1)) i3) i1 (i2)
-*)
-
-Fixpoint shift_substitution (A : formula) (i1 i2 : ivar) : formula :=
-match A with
-| fal => fal
-| equ v1 v2 => match nat_eqb v1 i1, nat_eqb v2 i1 with
-    | true, true => equ (v1 + i2) (v2 + i2)
-    | true, false => equ (v1 + i2) v2
-    | false, true => equ v1 (v2 + i2)
-    | false, false => equ v1 v2
-    end
-| imp B C => imp (shift_substitution B i1 i2) (shift_substitution C i1 i2)
-| univ B => univ (shift_substitution B (S i1) i2)
-| bnd o1 o2 B => bnd o1 o2 (shift_substitution B i1 i2)
-| prd vec pn pure => prd (vec_map (fun n => if nat_eqb n i1 then n + i2 else n) vec) pn pure
-end.
-
-
-Fixpoint substitution_depth (A : formula) (depth : nat) (i1 i2 : ivar) : formula :=
-match A with
-| fal => fal
-| equ v1 v2 => match nat_eqb v1 i1, nat_eqb v2 i1 with
-    | true, true => equ i2 i2
-    | true, false => equ i2 v2
-    | false, true => equ v1 i2
-    | false, false => equ v1 v2
-    end
-| imp B C => imp (substitution_depth B depth i1 i2) (substitution_depth C depth i1 i2)
-| univ B =>
-    (match nat_ltb depth i1, nat_ltb depth i2 with
-    | true, true => univ (substitution_depth B (S depth) i1 i2)
-    | _, _ => A
-    end)
-| bnd o1 o2 B => bnd o1 o2 (substitution_depth B depth i1 i2)
-| prd vec pn pure => prd (vec_map (fun n => if nat_eqb n i1 then i2 else n) vec) pn pure
-end.
-
-Fixpoint substitution (A : formula) (i1 i2 : ivar) : formula :=
-match A with
-| fal => fal
-| equ v1 v2 => match nat_eqb v1 i1, nat_eqb v2 i1 with
-    | true, true => equ i2 i2
-    | true, false => equ i2 v2
-    | false, true => equ v1 i2
-    | false, false => A
-    end
-| imp B C => imp (substitution B i1 i2) (substitution C i1 i2)
-| univ B => univ (substitution B i1 i2)
-| bnd o1 o2 B => bnd o1 o2 (substitution B i1 i2)
-| prd vec pn pure => prd (vec_map (fun n => if nat_eqb n i1 then i2 else n) vec) pn pure
-end.
-
-Lemma vec_map_ext {n : nat} :
-    forall (F G : nat -> nat),
-        F = G ->
-          forall (vec : nvec n),
-              vec_map F vec = vec_map G vec.
-Proof.
-intros F G FEQ vec.
-rewrite FEQ.
-reflexivity.
-Qed.
-
-Lemma vec_map_id {n : nat} :
-    forall (vec : nvec n),
-              vec_map (fun n => n) vec = vec.
-Proof.
-induction vec.
-reflexivity.
-unfold vec_map;
-fold @vec_map.
-rewrite IHvec.
-reflexivity.
-Qed.
-
-Lemma vec_map_app {n : nat} :
-    forall (F G : nat -> nat) (vec : nvec n),
-        vec_map F (vec_map G vec) = vec_map (fun n => (F (G n))) vec.
-Proof.
-intros F G.
-induction vec.
-reflexivity.
-unfold vec_map;
-fold @vec_map.
-rewrite IHvec.
-reflexivity.
-Qed.
-
-Lemma subst_depth_eq_refl : forall (A : formula) (n : nat) (i : ivar), substitution_depth A n i i = A.
-Proof.
-induction A;
-intros n' iv;
-unfold substitution_depth;
-fold substitution_depth;
-try rewrite IHA;
-try rewrite IHA1;
-try rewrite IHA2;
-try reflexivity.
-1 : case (nat_eqb i iv) eqn:EQ1;
-    case (nat_eqb i0 iv) eqn:EQ2;
-    try apply nat_eqb_eq in EQ1;
-    try apply nat_eqb_eq in EQ2;
-    subst;
-    reflexivity.
-1 : case (nat_ltb n' iv) eqn:EQ;
-    reflexivity.
-1 : assert ((fun n0 => if nat_eqb n0 iv then iv else n0) = (fun n => n)) as EQ.
-    { apply functional_extensionality.
-      intros x.
-      case (nat_eqb x iv) eqn:EQ.
-      apply nat_eqb_eq in EQ.
-      rewrite EQ.
-      all : reflexivity. }
-    rewrite (vec_map_ext _ _ EQ), vec_map_id.
-    reflexivity.
-Qed.
-
-Lemma subst_eq_refl : forall (A : formula) (i : ivar), substitution A i i = A.
-Proof.
-induction A;
-intros iv;
-unfold substitution;
-fold substitution;
-try rewrite IHA;
-try rewrite IHA1;
-try rewrite IHA2;
-try reflexivity.
-1 : case (nat_eqb i iv) eqn:EQ1;
-    case (nat_eqb i0 iv) eqn:EQ2;
-    try apply nat_eqb_eq in EQ1;
-    try apply nat_eqb_eq in EQ2;
-    subst;
-    reflexivity.
-1 : assert ((fun n0 => if nat_eqb n0 iv then iv else n0) = (fun n => n)) as EQ.
-    { apply functional_extensionality.
-      intros x.
-      case (nat_eqb x iv) eqn:EQ.
-      apply nat_eqb_eq in EQ.
-      rewrite EQ.
-      all : reflexivity. }
-    rewrite (vec_map_ext _ _ EQ), vec_map_id.
-    reflexivity.
-Qed.
-
-Lemma subst_forms_equiv_for_free_var_aux :
-    forall (phi : formula) (v1 v2 : ivar) (n : nat),
-        nat_ltb (form_depth phi + n) v1 = true ->
-            nat_ltb (form_depth phi + n) v2 = true ->
-                substitution_depth phi n v1 v2 = substitution phi v1 v2.
-Proof.
-induction phi;
-intros v1 v2 n' FV1 FV2;
-unfold substitution_depth;
-fold substitution_depth;
-unfold substitution;
-fold substitution;
-try reflexivity;
-unfold form_depth in *;
-fold form_depth in *;
-apply nat_ltb_lt in FV1, FV2.
-3 : rewrite IHphi.
-2 : assert (n' < v1 /\ n' < v2) as [LT1 LT2].
-2 : split; lia.
-2 : rewrite (nat_lt_ltb _ _ LT1), (nat_lt_ltb _ _ LT2), IHphi.  
-1 : rewrite IHphi1, IHphi2.
-all : try reflexivity;
-      apply nat_lt_ltb;
-      lia.
-Qed.
-
-Lemma subst_forms_equiv_for_free_var :
-    forall (phi : formula) (v1 v2 : ivar),
-        nat_ltb (form_depth phi) v1 = true ->
-            nat_ltb (form_depth phi) v2 = true ->
-                substitution_depth phi 0 v1 v2 = substitution phi v1 v2.
-Proof.
-intros phi v1 v2 LT1 LT2.
-apply subst_forms_equiv_for_free_var_aux;
-rewrite <- plus_n_O.
-apply LT1.
-apply LT2.
-Qed.
-
-Lemma nvec_case :
-    forall (n : nat) (P : nvec n -> Type),
-        (forall (pf : n = 0),
-            P (eq_rect 0 nvec Null n (eq_sym pf))) ->
-        (forall (m i : nat) (vec : nvec m) (pf : n = S m), P (eq_rect (S m) nvec (New i vec) n (eq_sym pf))) ->
-            (forall (vec : nvec n), P vec).
-Proof.
-intros n P BC IND vec.
-induction vec.
-apply (BC eq_refl).
-apply (IND _ _ _ eq_refl).
-Defined.
-
-Lemma nvec_0_null : forall (vec : nvec 0), vec = Null.
-Proof.
-apply nvec_case.
-- intros pf.
-  subst.
-  rewrite <- Eqdep_dec.eq_rect_eq_dec in * by apply nat_eq_dec.
-  reflexivity.
-- intros i m vec pf.
-  inversion pf.
-Qed.
-
-Lemma nvec_Sn_new : forall {n : nat} (vec : nvec (S n)), {subvec : nvec n & {m : nat & vec = New m subvec}}.
-Proof.
-intros n.
-apply nvec_case.
-- intros pf.
-  inversion pf.
-- intros i m vec pf.
-  inversion pf as [pf'].
-  subst.
-  rewrite <- Eqdep_dec.eq_rect_eq_dec in * by apply nat_eq_dec.
-  apply (existT _ vec (existT _ m eq_refl)).
-Defined.
-
-Lemma nvec_eqb_eq :
-    forall {n : nat} (vec1 vec2 : nvec n),
-        nvec_eqb vec1 vec2 = true ->
-            vec1 = vec2.
-Proof.
-induction n;
-intros vec1 vec2 EQB.
-- pose proof (nvec_0_null vec1).
-  pose proof (nvec_0_null vec2).
-  subst.
-  reflexivity.
-- pose proof (nvec_Sn_new vec1) as [vec3 [m1 EQ1]].
-  pose proof (nvec_Sn_new vec2) as [vec4 [m2 EQ2]].
-  subst.
-  apply and_bool_prop in EQB as [EQ1 EQ2].
-  apply nat_eqb_eq in EQ1.
-  subst.
-  rewrite (IHn _ _ EQ2).
-  reflexivity.
-Qed.
-
-Lemma nvec_eqb_sym :
-    forall {n1 n2 : nat} (vec1 : nvec n1) (vec2 : nvec n2),
-        nvec_eqb vec1 vec2 = nvec_eqb vec2 vec1.
-Proof.
-induction n1;
-destruct n2;
-intros vec1 vec2;
-try pose proof (nvec_0_null vec1);
-try pose proof (nvec_0_null vec2);
-try pose proof (nvec_Sn_new vec1) as [vec3 [m1 EQ1]];
-try pose proof (nvec_Sn_new vec2) as [vec4 [m2 EQ2]];
-subst;
-try reflexivity.
-unfold nvec_eqb;
-fold @nvec_eqb.
-rewrite nat_eqb_symm, IHn1.
-reflexivity.
-Qed.
-
-Lemma nvec_eqb_refl :
-    forall {n : nat} (vec : nvec n),
-        nvec_eqb vec vec = true.
-Proof.
-induction n;
-intros vec.
-- pose proof (nvec_0_null vec).
-  subst.
-  reflexivity.
-- pose proof (nvec_Sn_new vec) as [vec' [m EQ]].
-  subst.
-  unfold nvec_eqb;
-  fold @nvec_eqb.
-  rewrite nat_eqb_refl.
-  rewrite IHn.
-  reflexivity.
-Qed.
-
-Definition nvec_eq_dec {n : nat}: forall (a b : nvec n), {a = b} + {a <> b}.
-intros a b.
-case (nvec_eqb a b) eqn:EQ.
-- left. apply nvec_eqb_eq, EQ.
-- right.
-  intros FAL.
-  subst.
-  rewrite nvec_eqb_refl in EQ.
-  inversion EQ.
-Qed.
-
-Lemma nvec_eqb_type : 
-    forall {n1 n2 : nat} (vec1 : nvec n1) (vec2 : nvec n2),
-        nvec_eqb vec1 vec2 = true -> nat_eqb n1 n2 = true .
-Proof.
-intros n1 n2 vec1.
-revert n2.
-induction vec1;
-intros n2 vec2 EQB;
-destruct vec2;
-unfold nvec_eqb in EQB.
-- reflexivity.
-- inversion EQB.
-- inversion EQB.
-- unfold nvec_eqb in EQB;
-  fold @nvec_eqb in EQB.
-  apply and_bool_prop in EQB as [EQB1 EQB2].
-  apply (IHvec1 _ _ EQB2).
-Qed.
-
-Lemma pred_case :
-    forall (n : nat) (P : predicate n -> Type),
-        (forall (i : nat) (pf : n = 0),
-            P (eq_rect _ predicate (Nullary i) _ (eq_sym pf))) ->
-        (forall (m : nat) (i : nat) (prd : predicate m) (pf : n = S m),
-            P (eq_rect _ predicate (Succary i prd) _ (eq_sym pf))) ->
-        (forall (i : nat), P (Var i)) ->
-            (forall (pn : predicate n), P pn).
-Proof.
-intros n P BC IND VARS pn.
-induction pn.
-apply (BC _ eq_refl).
-apply (IND _ _ _ eq_refl).
-apply VARS.
-Qed.
 
 Lemma prd_eqb_sym :
-    forall {n1 n2 : nat} (pn1 : predicate n1) (pn2 : predicate n2),
+    forall (pn1 pn2 : predicate),
         prd_eqb pn1 pn2 = prd_eqb pn2 pn1. 
 Proof.
-intros n1 n2 pn1.
-revert n2.
 induction pn1;
-intros n2;
 destruct pn2;
 unfold prd_eqb;
 fold @prd_eqb;
 subst;
-try rewrite !nat_eqb_refl;
-try rewrite nat_eqb_symm;
-try rewrite (nat_eqb_symm v v0);
 try rewrite (nat_eqb_symm i i0);
-try rewrite IHpn1;
 reflexivity.
 Qed.
 
 Lemma prd_eqb_eq :
-    forall {n : nat} (pn1 pn2 : predicate n),
+    forall (pn1 pn2 : predicate),
         prd_eqb pn1 pn2 = true ->
             pn1 = pn2.
 Proof.
-intros n.
 induction pn1;
-intros pn2.
-- apply (pred_case 0 (fun (pn2 : predicate 0) => prd_eqb (Nullary i) pn2 = true -> (Nullary i) = pn2)).
-  + intros i1 pf EQB.
-    rewrite pf in EQB.
-    unfold eq_rect, eq_sym, prd_eqb, nat_eqb in EQB.
-    apply nat_eqb_eq in EQB.
-    subst.
-    pose proof (UIP_refl _ _ pf).
-    subst.
-    reflexivity.
-  + intros m i1 pn1 pf EQB.
-    inversion pf.
-  + intros i1 EQB.
-    inversion EQB.
-- apply (pred_case (S m) (fun (pn2 : predicate (S m)) => prd_eqb (Succary i pn1) pn2 = true -> (Succary i pn1) = pn2)).
-  + intros i1 pf EQB.
-    inversion pf.
-  + intros m2 i2 pn3 pf EQB.
-    inversion pf as [pf'].
-    subst.
-    pose proof (UIP_refl _ _ pf).
-    subst.
-    unfold eq_rect, eq_sym, prd_eqb in EQB;
-    fold @prd_eqb in EQB.
-    rewrite nat_eqb_refl in EQB.
-    apply and_bool_prop in EQB as [EQ1 EQ2].
-    apply nat_eqb_eq in EQ1.
-    specialize (IHpn1 _ EQ2) as EQ3.
-    subst.
-    reflexivity.
-  + intros i1 EQB.
-    unfold prd_eqb in EQB.
-    rewrite nat_eqb_refl in EQB.
-    inversion EQB.
-- apply (pred_case n (fun (pn2 : predicate n) => prd_eqb (Var i) pn2 = true -> (Var i) = pn2)).
-  + intros i1 pf EQB.
-    subst.
-    inversion EQB.
-  + intros m i1 pn1 pf EQB.
-    subst.
-    unfold eq_rect, eq_sym, prd_eqb in EQB.
-    rewrite nat_eqb_refl in EQB.
-    inversion EQB.
-  + intros i2 EQB.
-    unfold prd_eqb in EQB.
-    rewrite nat_eqb_refl in EQB.
-    apply nat_eqb_eq in EQB.
-    subst.
-    reflexivity.
+destruct pn2;
+intros EQ;
+unfold prd_eqb in EQ;
+try inversion EQ;
+try apply nat_eqb_eq in EQ;
+subst;
+reflexivity.
 Qed.
 
 Lemma prd_eqb_refl :
-    forall {n : nat} (pn : predicate n),
+    forall (pn : predicate),
         prd_eqb pn pn = true.
 Proof.
-intros n pn.
-induction pn;
+destruct pn;
 unfold prd_eqb;
 fold @prd_eqb;
 repeat rewrite nat_eqb_refl;
-try rewrite IHpn;
-try reflexivity.
+reflexivity.
 Qed.
 
-Lemma prd_eqb_type : 
-    forall {n1 n2 : nat} (pn1 : predicate n1) (pn2 : predicate n2),
-        prd_eqb pn1 pn2 = true -> nat_eqb n1 n2 = true .
-Proof.
-intros n1 n2 pn1 pn2 EQB.
-destruct pn1, pn2;
-subst;
-unfold prd_eqb, eq_rect, eq_sym in EQB;
-fold @prd_eqb in EQB.
-- reflexivity.
-- inversion EQB.
-- case (nat_eqb 0 n) eqn:EQ1;
-  inversion EQB.
-- inversion EQB.
-- case (nat_eqb (S m) (S m0)) eqn:EQ1.
-  reflexivity.
-  inversion EQB.
-- case (nat_eqb (S m) n) eqn:EQ1;
-  inversion EQB.
-- case (nat_eqb n 0) eqn:EQ1;
-  inversion EQB.
-- case (nat_eqb n (S m)) eqn:EQ1;
-  inversion EQB.
-- case (nat_eqb n n0) eqn:EQ1;
-  inversion EQB;
-  reflexivity.
-Qed.
-
-Definition prd_eq_dec {n : nat} : forall (a b : predicate n), {a = b} + {a <> b}.
+Definition prd_eq_dec : forall (a b : predicate), {a = b} + {a <> b}.
 intros a b.
 case (prd_eqb a b) eqn:EQ.
 - left. apply prd_eqb_eq, EQ.
@@ -635,19 +146,11 @@ try apply nat_eqb_eq in EQ as [];
 try apply nat_eqb_eq in EQ0 as [];
 try apply nat_eqb_eq in EQ1 as [].
 - reflexivity.
-- reflexivity.
 - rewrite (IHA1 _ EQ),(IHA2 _ EQ0).
-  reflexivity.
-- rewrite (IHA _ EQ').
   reflexivity.
 - rewrite (IHA _ EQ0).
   reflexivity.
-- apply and_bool_prop in EQ' as [EQ1 EQ2].
-  pose proof (prd_eqb_type _ _ EQ2) as EQ3.
-  apply nat_eqb_eq in EQ3.
-  subst.
-  apply nvec_eqb_eq in EQ1.
-  apply prd_eqb_eq in EQ2.
+- apply prd_eqb_eq in EQ'.
   subst.
   rewrite (UIP  _ _ _ e e0).
   reflexivity.
@@ -663,9 +166,8 @@ repeat rewrite nat_eqb_refl;
 try rewrite IHa;
 try rewrite IHa1;
 try rewrite IHa2;
-try reflexivity.
-rewrite nvec_eqb_refl.
-apply prd_eqb_refl.
+try rewrite prd_eqb_refl;
+reflexivity.
 Qed.
 
 Definition form_eq_dec : forall (a b : formula), {a = b} + {a <> b}.
@@ -678,463 +180,3 @@ case (form_eqb a b) eqn:EQ.
   rewrite form_eqb_refl in EQ.
   inversion EQ.
 Qed.
-
-Lemma shift_subst_neb_form_neb :
-    forall (phi1 phi2 : formula) (v1 v2 : ivar),
-        form_eqb (shift_substitution phi1 v1 v2) (shift_substitution phi2 v1 v2) = false ->
-            form_eqb phi1 phi2 = false.
-Proof.
-induction phi1;
-destruct phi2;
-intros v1 v2 EQ;
-unfold shift_substitution in *;
-fold shift_substitution in *;
-unfold form_eqb in *;
-fold form_eqb in *;
-try apply andb_false_elim in EQ as [EQ1 | EQ2];
-try rewrite (IHphi1 _ _ _ EQ);
-try rewrite (IHphi1 _ _ _ EQ2);
-try rewrite (IHphi1_1 _ _ _ EQ1);
-try rewrite (IHphi1_2 _ _ _ EQ2);
-try rewrite EQ1;
-try rewrite EQ2;
-try rewrite andb_false_r;
-try apply EQ;
-try reflexivity.
-- case (nat_eqb i v1) eqn:EQ1;
-  case (nat_eqb i0 v1) eqn:EQ2;
-  case (nat_eqb i1 v1) eqn:EQ3;
-  case (nat_eqb i2 v1) eqn:EQ4;
-  try apply nat_eqb_eq in EQ1;
-  try apply nat_eqb_eq in EQ2;
-  try apply nat_eqb_eq in EQ3;
-  try apply nat_eqb_eq in EQ4;
-  subst;
-  unfold form_eqb in EQ;
-  try rewrite nat_eqb_refl in *;
-  try rewrite andb_true_l in *;
-  try rewrite andb_true_r in *;
-  try rewrite EQ;
-  try rewrite EQ1;
-  try rewrite EQ2;
-  try rewrite nat_eqb_symm;
-  try rewrite EQ3;
-  try reflexivity.
-  apply EQ4.
-  rewrite (nat_eqb_symm i2 v1), EQ4.
-  all : apply andb_false_r.
-- case (nvec_eqb vec vec0) eqn:EQV.
-  pose proof (nvec_eqb_type _ _ EQV) as EQN.
-  apply nat_eqb_eq in EQN.
-  subst.
-  apply nvec_eqb_eq in EQV.
-  subst.
-  rewrite nvec_eqb_refl in EQ1.
-  inversion EQ1.
-  reflexivity.
-Qed.
-
-Fixpoint nvec_equiv {n1 n2 : nat} (vec1 : nvec n1) (vec2 : nvec n2) (diff : ivar) : bool :=
-match vec1, vec2 with
-| Null, Null => true
-| New v1 vec1', New v2 vec2' => (nat_eqb v1 v2 || nat_eqb (v1 + diff) v2) && nvec_equiv vec1' vec2' diff
-| _, _ => false
-end.
-
-Lemma nvec_equiv_0_eq {n : nat} :
-    forall (vec1 vec2 : nvec n),
-        nvec_equiv vec1 vec2 0 = true ->
-            vec1 = vec2.
-Proof.
-induction vec1.
-- apply (nvec_case _ (fun (vec2 : nvec 0) => nvec_equiv Null vec2 0 = true -> Null = vec2)).
-  + intros pf EQ.
-    rewrite (UIP_refl _ _ pf) in *.
-    reflexivity.
-  + intros m i vec pf EQ.
-    inversion pf.
-- apply (nvec_case _ (fun vec2 => nvec_equiv (New n vec1) vec2 0 = true -> (New n vec1) = vec2)).
-  + intros pf EQ'.
-    inversion pf.
-  + intros m' i vec2 pf EQ.
-    inversion pf as [pf'].
-    subst.
-    rewrite (UIP_refl _ _ pf) in *.
-    unfold eq_rect, eq_sym in *.
-    apply and_bool_prop in EQ as [EQ1 EQ2].
-    rewrite <- plus_n_O, orb_diag in EQ1.
-    apply nat_eqb_eq in EQ1.
-    subst.
-    rewrite (IHvec1 _ EQ2).
-    reflexivity.
-Qed.
-
-
-Lemma nvec_equiv_0_eqb {n1 n2 : nat} :
-    forall (vec1 : nvec n1) (vec2 : nvec n2),
-        nvec_equiv vec1 vec2 0 = nvec_eqb vec1 vec2.
-Proof.
-intros vec1.
-revert n2.
-induction vec1;
-induction vec2;
-unfold nvec_equiv;
-fold @nvec_equiv;
-unfold nvec_eqb;
-fold @nvec_eqb;
-try rewrite <- plus_n_O, orb_diag;
-try rewrite IHvec1;
-try reflexivity.
-Qed.
-
-Lemma nvec_vec_map_shift {n : nat} :
-    forall (vec : nvec n) (v1 v2 : ivar),
-        nvec_equiv vec (vec_map (fun m => if nat_eqb m v1 then m + v2 else m) vec) v2 = true.
-Proof.
-induction vec;
-intros v1 v2;
-unfold vec_map;
-fold @vec_map;
-unfold nvec_equiv;
-fold @nvec_equiv.
-reflexivity.
-rewrite IHvec.
-case (nat_eqb n v1) eqn:EQ;
-rewrite nat_eqb_refl;
-try rewrite orb_true_r;
-reflexivity.
-Qed.
-
-Lemma nvec_equiv_refl {n : nat} :
-    forall (vec : nvec n) (diff: ivar),
-        nvec_equiv vec vec diff = true.
-Proof.
-induction vec;
-intros diff;
-unfold nvec_equiv;
-fold @nvec_equiv;
-try rewrite IHvec;
-try rewrite nat_eqb_refl;
-reflexivity.
-Qed.
-
-Fixpoint form_equiv (A1 A2 : formula) (diff : ivar) : bool :=
-match A1, A2 with
-| fal, fal => true
-| equ v1 v2, equ v3 v4 => (nat_eqb v1 v3 || nat_eqb (v1 + diff) v3) && (nat_eqb v2 v4 || nat_eqb (v2 + diff) v4)
-| imp B1 C1, imp B2 C2 => form_equiv B1 B2 diff && form_equiv C1 C2 diff
-| univ B1, univ B2 => form_equiv B1 B2 diff
-| bnd lambda1 kappa1 B1, bnd lambda2 kappa2 B2 => nat_eqb lambda1 lambda2 && nat_eqb kappa1 kappa2 && form_equiv B1 B2 diff
-| prd vec1 pn1 _, prd vec2 pn2 _ => nvec_equiv vec1 vec2 diff && prd_eqb pn1 pn2
-| _, _ => false
-end.
-
-Lemma form_equiv_preserves_depth :
-    forall (A1 A2 : formula) (d : nat),
-        form_equiv A1 A2 d = true ->
-            form_depth A1 = form_depth A2.
-Proof.
-induction A1;
-destruct A2;
-intros d EQ;
-inversion EQ as [EQ'];
-unfold form_depth;
-fold form_depth;
-try apply and_bool_prop in EQ' as [EQ1 EQ2];
-try rewrite (IHA1 _ _ EQ');
-try rewrite (IHA1 _ _ EQ2);
-try rewrite (IHA1_1 _ _ EQ1);
-try rewrite (IHA1_2 _ _ EQ2);
-try reflexivity.
-Qed.
-
-Lemma form_equiv_preserves_ovars :
-    forall (A1 A2 : formula) (d : nat),
-        form_equiv A1 A2 d = true ->
-            vars_in A1 = vars_in A2.
-Proof.
-induction A1;
-destruct A2;
-intros d EQ;
-inversion EQ as [EQ'];
-unfold vars_in;
-fold vars_in;
-repeat apply and_bool_prop in EQ' as [EQ' ?EQ];
-try apply nat_eqb_eq in EQ';
-try apply nat_eqb_eq in EQ1;
-subst;
-try rewrite (IHA1 _ _ EQ');
-try rewrite (IHA1 _ _ EQ0);
-try rewrite (IHA1_1 _ _ EQ');
-try rewrite (IHA1_2 _ _ EQ0);
-try reflexivity.
-Qed.
-
-Lemma form_equiv_0_eq : 
-    forall (phi1 phi2 : formula),
-        form_equiv phi1 phi2 0 = form_eqb phi1 phi2.
-Proof.
-induction phi1;
-destruct phi2;
-unfold form_equiv;
-fold form_equiv;
-unfold form_eqb;
-fold form_eqb;
-try rewrite IHphi1;
-try rewrite IHphi1_1, IHphi1_2;
-try rewrite nat_eqb_refl;
-try rewrite nvec_equiv_0_eqb;
-try rewrite <- !plus_n_O, !orb_diag;
-reflexivity.
-Qed.
-
-Lemma form_equiv_diff_shift_subst :
-    forall (phi : formula) (v1 v2 : ivar),
-        form_equiv phi (shift_substitution phi v1 v2) v2 = true.
-Proof. 
-induction phi;
-intros v1 v2;
-unfold shift_substitution;
-fold shift_substitution;
-unfold form_equiv;
-fold form_equiv;
-try rewrite !nat_eqb_refl;
-try rewrite prd_eqb_refl;
-try rewrite IHphi;
-try rewrite IHphi1, IHphi2;
-try rewrite nvec_vec_map_shift;
-try reflexivity.
-case (nat_eqb i v1) eqn:EQ1;
-case (nat_eqb i0 v1) eqn:EQ2;
-try apply nat_eqb_eq in EQ1;
-try apply nat_eqb_eq in EQ2;
-subst;
-try rewrite !nat_eqb_refl;
-try rewrite !orb_true_l;
-try rewrite !orb_true_r;
-reflexivity.
-Qed.
-
-Lemma shift_subst_idem :
-    forall (phi : formula) (v1 v2 : ivar),
-        shift_substitution (shift_substitution phi v1 v2) v1 v2 = shift_substitution phi v1 v2.
-Proof.
-induction phi;
-intros v1 v2;
-unfold shift_substitution;
-fold shift_substitution;
-try rewrite IHphi;
-try rewrite IHphi1, IHphi2;
-try reflexivity.
-- case (nat_eqb i v1) eqn:EQ1;
-  case (nat_eqb i0 v1) eqn:EQ2;
-  try apply nat_eqb_eq in EQ1;
-  try apply nat_eqb_eq in EQ2;
-  subst;
-  unfold shift_substitution;
-  fold shift_substitution;
-  try rewrite EQ1;
-  try rewrite EQ2;
-  case (nat_eqb (v1 + v2) v1) eqn:EQ3;
-  try apply nat_eqb_eq in EQ3;
-  try rewrite !EQ3;
-  reflexivity.
-- rewrite vec_map_app.
-  rewrite <- (vec_map_ext (fun n0 => if nat_eqb n0 v1 then n0 + v2 else n0)).
-  reflexivity.
-  apply functional_extensionality.
-  intros m.
-  case (nat_eqb m v1) eqn:EQ.
-  + apply nat_eqb_eq in EQ;
-    subst.
-    destruct v2.
-    rewrite <- !plus_n_O, nat_eqb_refl.
-    reflexivity.
-    case (nat_eqb (v1 + S v2) v1) eqn:EQ.
-    apply nat_eqb_eq in EQ.
-    rewrite !EQ.
-    reflexivity.
-    reflexivity.
-  + rewrite EQ.
-    reflexivity.
-Qed.
-
-Lemma form_equiv_refl :
-    forall (phi : formula) (d : nat),
-        form_equiv phi phi d = true.
-Proof.
-induction phi;
-intros d;
-unfold form_equiv;
-fold form_equiv;
-try rewrite !nat_eqb_refl;
-try rewrite prd_eqb_refl;
-try rewrite !orb_true_l;
-try rewrite IHphi;
-try rewrite IHphi1, IHphi2;
-try rewrite nvec_equiv_refl;
-try reflexivity.
-Qed.
-
-(*
-Fixpoint sig_subst (a : formula) (sig : ovar -> ovar) : formula :=
-match a with
-| fal => fal
-| equ v1 v2 => equ v1 v2
-| imp a1 a2 =>  imp (sig_subst a1 sig) (sig_subst a2 sig)
-| univ v a => univ v (sig_subst a sig)
-| bnd o1 o2 a => bnd o1 (sig o2) (sig_subst a (fun o => if nat_eq_dec o o1 then o else sig o))
-| prd pn pure => prd pn pure
-end.
-
-Lemma sig_subst_id :
-    forall (phi : formula),
-        sig_subst phi (fun o => o) = phi.
-Proof.
-induction phi;
-unfold sig_subst;
-fold sig_subst;
-try reflexivity.
-rewrite IHphi1, IHphi2.
-reflexivity.
-rewrite IHphi.
-reflexivity.
-assert ((fun o1 : ovar => if nat_eq_dec o1 o then o1 else o1) = fun o2 => o2) as FEQ.
-{ apply functional_extensionality.
-  intros o1.
-  case nat_eq_dec;
-  reflexivity. }
-rewrite FEQ, IHphi.
-reflexivity.
-Qed.
-
-Lemma sig_subst_ext :
-    forall (phi : formula) (f g : ovar -> ovar),
-        f = g ->
-            sig_subst phi f = sig_subst phi g.
-Proof.
-intros phi f g FEQ.
-rewrite FEQ.
-reflexivity.
-Qed.
-
-Lemma sig_subst_coherent_bi_is_inj {OC1 OC2 : constraint} :
-    forall (phi1 phi2 : formula) (sig : constraint_type OC1 -> constraint_type OC2),
-        coherent_bijection sig ->
-            incl (vars_in phi1) (OC_list OC1) ->
-                incl (vars_in phi2) (OC_list OC1) ->
-                    phi1 = phi2 <-> sig_subst phi1 (sig_generalise sig) = sig_subst phi2 (sig_generalise sig).
-Proof.
-induction phi1;
-destruct phi2;
-intros sig COH SUB1 SUB2;
-split;
-intros EQ;
-try inversion EQ;
-subst;
-try reflexivity.
-- rewrite (proj2 (IHphi1_1 phi2_1 sig COH (fun o IN => (SUB1 _ (in_or_app _ _ _ (or_introl IN)))) (fun o IN => (SUB2 _ (in_or_app _ _ _ (or_introl IN))))) H0).
-  rewrite (proj2 (IHphi1_2 phi2_2 sig COH (fun o IN => (SUB1 _ (in_or_app _ _ _ (or_intror IN)))) (fun o IN => (SUB2 _ (in_or_app _ _ _ (or_intror IN))))) H1).
-  reflexivity.
-- rewrite (proj2 (IHphi1 phi2 sig COH (fun o IN => (SUB1 _ IN)) (fun o IN => (SUB2 _ IN))) H1).
-  reflexivity.
-- unfold vars_in in *;
-  fold vars_in in *.
-  unfold sig_generalise in H1.
-  case (in_dec nat_eq_dec o0 (OC_list OC1)) as [IN1 | FAL].
-  case (in_dec nat_eq_dec o2 (OC_list OC1)) as [IN2 | FAL].
-  + apply constraint_type_eq_proj in H1.
-    apply (coherent_bijective_is_injective _ COH) in H1.
-    inversion H1.
-    subst.
-    pose proof (proof_irrelevance _ IN1 IN2).
-    subst.
-    assert (incl (vars_in phi1) (OC_list OC1)) as SUB1'.
-    admit.
-    assert (incl (vars_in phi2) (OC_list OC1)) as SUB2'.
-    admit.
-    case (in_dec nat_eq_dec o1 (OC_list OC1)) as [IN1 | NIN1].
-    assert ((fun o : ovar => if nat_eq_dec o o1 then o else (sig_generalise sig o)) = sig_generalise (fun o => if nat_eq_dec (projT1 o) o1 then (existT (OC_elt OC2) (projT1 o) ((fst (fst (fst COH))) _)) else sig o)) as EQF.
-    rewrite (proj2 (IHphi1 _ _ _ SUB1' SUB2')).
-    admit.
-  + contradiction (FAL (SUB2 _ (or_introl eq_refl))).
-  + contradiction (FAL (SUB1 _ (or_introl eq_refl))).
-Qed.
-(*
-Lemma sig_applicable_sig_inverse {OC1 OC2 : constraint} (sig : constraint_type OC1 -> constraint_type OC2) :
-    forall (phi : formula),
-        incl (vars_in phi) (OC_list OC2) ->
-            coherent_bijection sig -> 
-                sig_subst (sig_subst phi (sig_inverse sig)) (sig_generalise sig) = phi.
-Proof.
-intros phi.
-revert sig.
-induction phi;
-intros sig SUB COH;
-try reflexivity.
-- unfold sig_subst;
-  fold sig_subst.
-  unfold vars_in in *;
-  fold vars_in in *.
-  rewrite IHphi1, IHphi2;
-  try assumption.
-  reflexivity.
-  refine (fun o IN => SUB _ (in_or_app _ _ _ (or_intror IN))).
-  refine (fun o IN => SUB _ (in_or_app _ _ _ (or_introl IN))).
-- unfold sig_subst;
-  fold sig_subst.
-  unfold vars_in in *;
-  fold vars_in in *.
-  rewrite IHphi.
-  reflexivity.
-  apply SUB.
-  apply COH.
-- unfold sig_subst;
-  fold sig_subst.
-  unfold vars_in in *;
-  fold vars_in in *.
-  rewrite (coherent_bijection_sig_inverse _ COH _ (SUB _ (or_introl eq_refl))).
-  assert ((sig_subst (sig_subst phi (fun o1 : ovar => if nat_eq_dec o1 o then o1 else sig_inverse sig o1)) (fun o1 : ovar => if nat_eq_dec o1 o then o1 else sig_generalise sig o1)) = sig_subst phi (fun o1 : ovar => o1)) as EQ.
-  { case (in_dec nat_eq_dec o (OC_list OC2)) as [IN | NIN].
-    + assert ((fun o1 : ovar => if nat_eq_dec o1 o then o1 else sig_inverse sig o1) = sig_inverse (fun o1 : constraint_type OC1 => if nat_eq_dec (projT1 o1) o then (existT _ o IN) else sig o1)) as EQ1.
-      { admit. }
-      assert ((fun o1 : ovar => if nat_eq_dec o1 o then o1 else sig_generalise sig o1) = sig_generalise (fun o1 : constraint_type OC1 => if nat_eq_dec (projT1 o1) o then (existT _ o IN) else sig o1)) as EQ2.
-      { admit. }
-      rewrite EQ1, EQ2, IHphi, sig_subst_id.
-      reflexivity.
-      admit.
-      destruct COH as [[[INJ SUR] REL_iff] PREC].
-      repeat split.
-      * intros lambda.
-        case (nat_eq_dec (projT1 lambda) o) as [EQ | NE].
-        apply IN.
-        apply INJ.
-      * intros [lambda IN'].
-        case (nat_eq_dec lambda o) as [EQ | NE].
-        --  refine (existT _ (existT _ o _) _).
-            unfold projT1.
-            case (nat_eq_dec o o) as [_ | FAL].
-            subst.
-            rewrite (proof_irrelevance _ IN IN').
-            reflexivity.
-            contradiction (FAL eq_refl).
-        --  destruct (SUR (existT _ lambda IN')) as [[kappa IN''] EQ].
-            refine (existT _ (existT _ kappa _) _).
-            unfold projT1.
-            rewrite EQ.
-            
-    + assert ((fun o1 : ovar => if nat_eq_dec o1 o then o1 else sig_inverse sig o1) = sig_inverse sig) as EQ1.
-      { admit. }
-      assert ((fun o1 : ovar => if nat_eq_dec o1 o then o1 else sig_generalise sig o1) = sig_generalise sig) as EQ2.
-      { admit. }
-      rewrite EQ1, EQ2, IHphi, sig_subst_id.
-      reflexivity.
-      admit.
-      apply COH.
-      
-    admit. }
-  rewrite EQ, sig_subst_id.
-  reflexivity.
-Admitted.
-*)
-*)
