theories/Logic/inverse_bnd_l.v
@@ -1,0 +1,909 @@
+From Cyclic_PA.Maths Require Import naturals.
+From Cyclic_PA.Maths Require Import lists.
+From Cyclic_PA.Maths Require Import ordinals.
+
+From Cyclic_PA.Logic Require Import definitions.
+From Cyclic_PA.Logic Require Import constraints.
+From Cyclic_PA.Logic Require Import fol.
+From Cyclic_PA.Logic Require Import proof_trees.
+From Cyclic_PA.Logic Require Import substitute.
+
+Require Import List.
+Require Import Bool.
+Require Import Lia.
+Import ListNotations.
+
+Definition bnd_left_inv_formula (phi A : formula) (lambda kappa : ovar) (b : bool) : formula := formula_sub phi (bnd lambda kappa A) A b.
+
+Definition bnd_left_inv_batch (gamma : list formula) (A : formula) (lambda kappa : ovar) (S : subst_ind) : list formula := batch_sub gamma (bnd lambda kappa A) A S.
+
+Fixpoint ptree_bnd_l_inv_fit
+  (P : ptree) (A : formula) (lambda kappa : ovar) (S : subst_ind) : ptree :=
+let REC := (fun PT SI => (ptree_bnd_l_inv_fit PT A lambda kappa SI)) in
+match P, S with
+| bot, _ => P
+
+| pred pn pure, _ => P
+
+| loop_head OC gamma delta alpha P_Target, _ => loop_head OC (bnd_left_inv_batch gamma A lambda kappa S) delta alpha (REC P_Target S)
+
+| @con_l OC gamma delta phi alpha P', s :: S' => @con_l OC (bnd_left_inv_batch gamma A lambda kappa S') delta (bnd_left_inv_formula phi A lambda kappa s) alpha (REC P' (s :: s :: S'))
+
+| @con_r OC gamma delta phi alpha P', _ => @con_r OC (ptree_left (REC P' S)) delta phi alpha (REC P' S)
+
+| @ex_l OC gamma delta n alpha P', _ => @ex_l OC (ptree_left (REC P' (unbury S n))) delta n alpha (REC P'(unbury S n))
+
+| @ex_r OC gamma delta n alpha P', _ => @ex_r OC (ptree_left (REC P' S)) delta n alpha (REC P' S)
+
+
+| @wkn_l OC gamma delta phi alpha P', s :: S' => @wkn_l OC (bnd_left_inv_batch gamma A lambda kappa S') delta (bnd_left_inv_formula phi A lambda kappa s) alpha (REC P' S')
+
+| @wkn_r OC gamma delta phi alpha P', _ => @wkn_r OC (ptree_left (REC P' S)) delta phi alpha (REC P' S)
+
+| @rst OC gamma delta kappa alpha P', _ => @rst OC (ptree_left (REC P' S)) delta kappa alpha (REC P' S)
+
+| @bnd_l OC gamma delta phi eta iota alpha P', s :: S' => match nat_eqb eta lambda, nat_eqb iota kappa, form_eqb phi A, s with
+    | true, true, true, true => REC P' (false :: S')
+    | _, _, _, _ => @bnd_l OC (bnd_left_inv_batch gamma A lambda kappa S') delta phi eta iota alpha (REC P' (false :: S'))
+    end
+
+| @bnd_r OC gamma delta phi eta iota alpha P', _ => @bnd_r OC (ptree_left (REC P' S)) delta phi eta iota alpha (REC P' S)
+
+| @imp_l OC gamma delta phi psi alpha1 alpha2 P1 P2, s :: S' =>  @imp_l OC (bnd_left_inv_batch gamma A lambda kappa S') delta phi psi alpha1 alpha2 (REC P1 (false :: S')) (REC P2 S')
+
+| @imp_r OC gamma delta phi psi alpha P', _ => @imp_r OC (bnd_left_inv_batch gamma A lambda kappa S) delta phi psi alpha (REC P' (false :: S))
+
+| @cut OC gamma delta phi alpha1 alpha2 P1 P2, _ => @cut OC (bnd_left_inv_batch gamma A lambda kappa S) delta phi alpha1 alpha2 (REC P1 S) (REC P2 (false :: S))
+
+| _ , _ => P
+end.
+
+Definition ptree_bnd_l_inv (P : ptree) (A : formula) (lambda kappa : ovar) (S : subst_ind) : ptree :=
+match nat_eqb (length (ptree_left P)) (length S) with
+| true => ptree_bnd_l_inv_fit P A lambda kappa S
+| false => P
+end.
+
+Lemma ptree_bnd_l_inv_fit_true :
+    forall {P : ptree} {A : formula} {lambda kappa : ovar},
+        forall {S : subst_ind},
+            nat_eqb (length (ptree_left P)) (length S) = true ->
+                (ptree_bnd_l_inv_fit P A lambda kappa S) = (ptree_bnd_l_inv P A lambda kappa S).
+Proof. intros P A lambda kappa S EQ. unfold ptree_bnd_l_inv. rewrite EQ. reflexivity. Qed.
+
+Lemma ptree_bnd_l_inv_left :
+    forall (P : ptree) (A : formula) (lambda kappa : ovar),
+        struct_valid P ->
+            forall (S : subst_ind),
+                ptree_left (ptree_bnd_l_inv P A lambda kappa S) =
+                    (bnd_left_inv_batch (ptree_left P) A lambda kappa S).
+Proof.
+intros P A lambda kappa.
+induction P;
+try intros PSV S;
+unfold ptree_bnd_l_inv;
+unfold bnd_left_inv_batch, batch_sub;
+case nat_eqb eqn:EQ;
+try reflexivity;
+unfold ptree_height;
+fold ptree_height;
+unfold ptree_bnd_l_inv_fit;
+fold ptree_bnd_l_inv_fit;
+unfold ptree_left in EQ;
+fold ptree_left in EQ.
+
+1-2 : destruct PSV.
+3 : destruct PSV as [[PSV [PG_app PD_app]] [PBot | [[[[PRec PG] PD] POC] PDeg]]].
+5-10 : destruct PSV as [[[[[PSV [PG_app PD_app]] PG] PD] POC] PDeg].
+11 : destruct PSV as [[[[[[[PSV [PG_app PD_app]] PG] PD] KNING] KNIND] [KIN POC]] PDeg].
+12 : destruct PSV as [[[[[[PSV [PG_app PD_app]] PG] PD] POC] POC_rel] PDeg].
+13 : destruct PSV as [[[[[[PSV [PG_app PD_app]] PG] PD] [NEW [KIN POC]]] [NING NIND]] PDeg].
+14 : destruct PSV as [[[[[[[[[[P1SV P2SV] [PG_app PD_app]] P1G] P1D] P1OC] P2G] P2D] P2OC] PDeg1] PDeg2].
+15 : destruct PSV as [[[[[PSV [PG_app PD_app]] PG] PD] POC] PDeg].
+16 : destruct PSV as [[[[[[[[[[P1SV P2SV] [PG_app PD_app]] P1G] P1D] P1OC] P2G] P2D] P2OC] PDeg1] PDeg2].
+
+all : subst;
+      unfold ptree_left;
+      unfold batch_sub_fit;
+      fold @batch_sub_fit.
+
+all : try rewrite (batch_sub_fit_true EQ);
+      try rewrite (ptree_bnd_l_inv_fit_true EQ);
+      unfold bnd_left_inv_batch;
+      try apply (IHP PSV);
+      try reflexivity.
+
+1-2 : destruct S;
+      reflexivity.
+
+2 : { fold (ptree_left (ptree_bnd_l_inv_fit P A lambda kappa (unbury S n))).
+      rewrite ptree_bnd_l_inv_fit_true, <- batch_bury_comm, (IHP PSV).
+      reflexivity.
+      rewrite bury_length, <- (@bury_unbury _ S n), bury_length in EQ.
+      apply EQ. }
+
+all : destruct S as [ | b S];
+      inversion EQ as [EQ'];
+      unfold length in *;
+      fold (@length bool) (@length formula) in *.
+
+3 : case (nat_eqb lambda0 lambda) eqn:EQL;
+    try apply nat_eqb_eq in EQL.
+3 : case (nat_eqb kappa0 kappa) eqn:EQK;
+    try apply nat_eqb_eq in EQK.
+3 : case (form_eqb phi A) eqn:EQF;
+    try apply form_eqb_eq in EQF.
+3 : destruct b.
+
+
+all : subst;
+      unfold ptree_left;
+      try fold (ptree_left P);
+      try fold (ptree_left P2);
+      unfold batch_sub, batch_sub_fit;
+      fold batch_sub_fit;
+      try rewrite batch_sub_fit_true;
+      try rewrite PG;
+      try rewrite EQ';
+      try rewrite EQ;
+      try apply EQ;
+      try reflexivity.
+
+1 : fold (ptree_left (ptree_bnd_l_inv_fit P A lambda kappa (false :: S))).
+    rewrite ptree_bnd_l_inv_fit_true, (IHP PSV).
+    rewrite PG.
+    unfold formula_sub, bnd_left_inv_batch, batch_sub, batch_sub_fit.
+    fold batch_sub_fit.
+    unfold length;
+    fold (@length bool) (@length formula).
+    rewrite EQ, EQ', form_eqb_refl.
+    unfold formula_sub.
+    case (form_eqb);
+    reflexivity.
+    rewrite PG.
+    apply EQ.
+
+1 : unfold bnd_left_inv_batch, batch_sub, batch_sub_fit at 1;
+    fold batch_sub_fit.
+    rewrite EQ', formula_sub_false.
+    reflexivity.
+
+all  : unfold formula_sub, form_eqb, bnd_left_inv_batch, batch_sub, batch_sub_fit at 1;
+    fold batch_sub_fit form_eqb;
+    try rewrite EQ';
+    try rewrite !nat_eqb_refl;
+    try rewrite EQL;
+    try rewrite EQK;
+    try rewrite EQF;
+    try rewrite !andb_false_r;
+    try rewrite !andb_false_l;
+    try reflexivity.
+Qed.
+
+Lemma ptree_bnd_l_inv_right :
+    forall (P : ptree) (A : formula) (lambda kappa : ovar),
+        struct_valid P ->
+            forall (S : subst_ind),
+                ptree_right (ptree_bnd_l_inv P A lambda kappa S) =
+                   (ptree_right P).
+Proof.
+intros P A lambda kappa.
+induction P;
+try intros PSV S;
+unfold ptree_bnd_l_inv;
+unfold bnd_left_inv_batch, batch_sub.
+
+1-2 : destruct PSV.
+3 : destruct PSV as [[PSV [PG_app PD_app]] [PBot | [[[[PRec PG] PD] POC] PDeg]]].
+5-10 : destruct PSV as [[[[[PSV [PG_app PD_app]] PG] PD] POC] PDeg].
+11 : destruct PSV as [[[[[[[PSV [PG_app PD_app]] PG] PD] KNING] KNIND] [KIN POC]] PDeg].
+12 : destruct PSV as [[[[[[PSV [PG_app PD_app]] PG] PD] POC] POC_rel] PDeg].
+13 : destruct PSV as [[[[[[PSV [PG_app PD_app]] PG] PD] [NEW [KIN POC]]] [NING NIND]] PDeg].
+14 : destruct PSV as [[[[[[[[[[P1SV P2SV] [PG_app PD_app]] P1G] P1D] P1OC] P2G] P2D] P2OC] PDeg1] PDeg2].
+15 : destruct PSV as [[[[[PSV [PG_app PD_app]] PG] PD] POC] PDeg].
+16 : destruct PSV as [[[[[[[[[[P1SV P2SV] [PG_app PD_app]] P1G] P1D] P1OC] P2G] P2D] P2OC] PDeg1] PDeg2].
+
+all : subst; 
+      case nat_eqb eqn:EQ;
+      try reflexivity;
+      unfold ptree_bnd_l_inv_fit;
+      fold ptree_bnd_l_inv_fit;
+      unfold ptree_left in EQ;
+      fold ptree_left in EQ.
+
+all : destruct S as [ | b S];
+      inversion EQ;
+      try case (nat_eqb lambda0 lambda) eqn:EQL;
+      try case (nat_eqb kappa0 kappa) eqn:EQK;
+      try case (form_eqb phi A) eqn:EQF;
+      destruct b;
+      try reflexivity.
+
+1 : rewrite ptree_bnd_l_inv_fit_true.
+    apply (IHP PSV).
+    rewrite PG.
+    apply EQ.
+Qed.
+
+Lemma ptree_bnd_l_inv_constraint :
+    forall (P : ptree) (A : formula) (lambda kappa : ovar),
+        struct_valid P ->
+            forall (S : subst_ind),
+                ptree_constraint (ptree_bnd_l_inv P A lambda kappa S) =
+                   (ptree_constraint P).
+Proof.
+intros P A lambda kappa.
+induction P;
+try intros PSV S;
+unfold ptree_bnd_l_inv;
+unfold bnd_left_inv_batch, batch_sub.
+
+1-2 : destruct PSV.
+3 : destruct PSV as [[PSV [PG_app PD_app]] [PBot | [[[[PRec PG] PD] POC] PDeg]]].
+5-10 : destruct PSV as [[[[[PSV [PG_app PD_app]] PG] PD] POC] PDeg].
+11 : destruct PSV as [[[[[[[PSV [PG_app PD_app]] PG] PD] KNING] KNIND] [KIN POC]] PDeg].
+12 : destruct PSV as [[[[[[PSV [PG_app PD_app]] PG] PD] POC] POC_rel] PDeg].
+13 : destruct PSV as [[[[[[PSV [PG_app PD_app]] PG] PD] [NEW [KIN POC]]] [NING NIND]] PDeg].
+14 : destruct PSV as [[[[[[[[[[P1SV P2SV] [PG_app PD_app]] P1G] P1D] P1OC] P2G] P2D] P2OC] PDeg1] PDeg2].
+15 : destruct PSV as [[[[[PSV [PG_app PD_app]] PG] PD] POC] PDeg].
+16 : destruct PSV as [[[[[[[[[[P1SV P2SV] [PG_app PD_app]] P1G] P1D] P1OC] P2G] P2D] P2OC] PDeg1] PDeg2].
+
+all : subst; 
+      case nat_eqb eqn:EQ;
+      try reflexivity;
+      unfold ptree_bnd_l_inv_fit;
+      fold ptree_bnd_l_inv_fit;
+      unfold ptree_left in EQ;
+      fold ptree_left in EQ.
+
+all : destruct S as [ | b S];
+      inversion EQ;
+      try case (nat_eqb lambda0 lambda) eqn:EQL;
+      try case (nat_eqb kappa0 kappa) eqn:EQK;
+      try case (form_eqb phi A) eqn:EQF;
+      destruct b;
+      try reflexivity.
+
+1 : rewrite ptree_bnd_l_inv_fit_true.
+    apply (IHP PSV).
+    rewrite PG.
+    apply EQ.
+Qed.
+
+Lemma ptree_bnd_l_inv_deg :
+    forall (P : ptree) (A : formula) (lambda kappa : ovar),
+        struct_valid P ->
+            forall (S : subst_ind),
+                ptree_deg (ptree_bnd_l_inv P A lambda kappa S) =
+                   (ptree_deg P).
+Proof.
+intros P A lambda kappa.
+induction P;
+try intros PSV S;
+unfold ptree_bnd_l_inv;
+unfold bnd_left_inv_batch, batch_sub.
+
+1-2 : destruct PSV.
+3 : destruct PSV as [[PSV [PG_app PD_app]] [PBot | [[[[PRec PG] PD] POC] PDeg]]].
+5-10 : destruct PSV as [[[[[PSV [PG_app PD_app]] PG] PD] POC] PDeg].
+11 : destruct PSV as [[[[[[[PSV [PG_app PD_app]] PG] PD] KNING] KNIND] [KIN POC]] PDeg].
+12 : destruct PSV as [[[[[[PSV [PG_app PD_app]] PG] PD] POC] POC_rel] PDeg].
+13 : destruct PSV as [[[[[[PSV [PG_app PD_app]] PG] PD] [NEW [KIN POC]]] [NING NIND]] PDeg].
+14 : destruct PSV as [[[[[[[[[[P1SV P2SV] [PG_app PD_app]] P1G] P1D] P1OC] P2G] P2D] P2OC] PDeg1] PDeg2].
+15 : destruct PSV as [[[[[PSV [PG_app PD_app]] PG] PD] POC] PDeg].
+16 : destruct PSV as [[[[[[[[[[P1SV P2SV] [PG_app PD_app]] P1G] P1D] P1OC] P2G] P2D] P2OC] PDeg1] PDeg2].
+
+all : subst; 
+      case nat_eqb eqn:EQ;
+      try reflexivity;
+      unfold ptree_bnd_l_inv_fit;
+      fold ptree_bnd_l_inv_fit;
+      unfold ptree_left in EQ;
+      fold ptree_left in EQ.
+
+all : destruct S as [ | b S];
+      inversion EQ;
+      try case (nat_eqb lambda0 lambda) eqn:EQL;
+      try case (nat_eqb kappa0 kappa) eqn:EQK;
+      try case (form_eqb phi A) eqn:EQF;
+      destruct b;
+      try reflexivity.
+
+1 : rewrite ptree_bnd_l_inv_fit_true.
+    apply (IHP PSV).
+    rewrite PG.
+    apply EQ.
+Qed.
+
+Lemma bnd_l_formula_inv_vars :
+    forall (phi : formula) (A : formula) (lambda kappa : ovar) (b : bool) (OC : constraint),
+        OC_rel OC lambda kappa = true ->
+            incl (vars_in phi) (OC_list OC) ->
+                incl (vars_in (bnd_left_inv_formula phi A lambda kappa b)) (OC_list OC).
+Proof.
+intros phi A lambda kappa b OC REL SUB o IN.
+unfold bnd_left_inv_formula, formula_sub in IN.
+case form_eqb eqn:EQF.
+destruct b.
+apply form_eqb_eq in EQF.
+subst.
+case (nat_eq_dec o lambda) as [EQ | NE].
+subst.
+apply (OC_null _ _ _ REL).
+apply SUB.
+apply (or_intror (in_in_remove _ _ NE IN)).
+all : apply SUB, IN.
+Qed.
+
+Lemma ptree_bnd_l_inv_vars :
+    forall (gamma : list formula) (A : formula) (lambda kappa : ovar) (S : subst_ind) (OC : constraint),
+        OC_rel OC lambda kappa = true ->
+            incl (flat_map vars_in gamma) (OC_list OC) ->
+                incl (flat_map vars_in (bnd_left_inv_batch gamma A lambda kappa S)) (OC_list OC).
+Proof.
+induction gamma;
+intros A lambda kappa S OC REL SUB;
+unfold bnd_left_inv_batch, batch_sub, batch_sub_fit;
+fold batch_sub_fit;
+destruct S;
+unfold length, nat_eqb;
+fold (@length formula) (@length bool) nat_eqb.
+4 : case nat_eqb eqn:EQN.
+1,2,3,5 : apply SUB.
+unfold flat_map;
+fold (flat_map vars_in).
+rewrite (batch_sub_fit_true EQN).
+fold (bnd_left_inv_batch gamma A lambda kappa S).
+apply incl_app_inv in SUB as [SUB1 SUB2].
+apply (incl_app (bnd_l_formula_inv_vars _ _ _ _ _ _ REL SUB1) (IHgamma _ _ _ _ _ REL SUB2)).
+Qed.
+
+
+Lemma bnd_l_formula_inv_vars_sub :
+    forall (phi : formula) (A : formula) (lambda kappa : ovar) (b : bool),
+        incl (vars_in (bnd_left_inv_formula phi A lambda kappa b)) (lambda :: (vars_in phi)).
+Proof.
+intros phi A lambda kappa b o IN.
+unfold bnd_left_inv_formula, formula_sub in IN.
+case form_eqb eqn:EQF.
+destruct b.
+apply form_eqb_eq in EQF.
+subst.
+case (nat_eq_dec o lambda) as [EQ | NE].
+subst.
+apply (or_introl eq_refl).
+apply (or_intror (or_intror (in_in_remove _ _ NE IN))).
+all : apply (or_intror IN).
+Qed.
+
+Lemma ptree_bnd_l_inv_vars_sub :
+    forall (gamma : list formula) (A : formula) (lambda kappa : ovar) (S : subst_ind),
+        incl (flat_map vars_in (bnd_left_inv_batch gamma A lambda kappa S)) (lambda :: (flat_map vars_in gamma)).
+Proof.
+induction gamma;
+intros A lambda kappa S;
+unfold bnd_left_inv_batch, batch_sub, batch_sub_fit;
+fold batch_sub_fit;
+destruct S;
+unfold length, nat_eqb;
+fold (@length formula) (@length bool) nat_eqb.
+4 : case nat_eqb eqn:EQN.
+1,2,3,5 : intros o IN;
+          apply or_intror, IN.
+unfold flat_map;
+fold (flat_map vars_in).
+rewrite (batch_sub_fit_true EQN).
+fold (bnd_left_inv_batch gamma A lambda kappa S).
+refine (incl_tran (incl_app_app (bnd_l_formula_inv_vars_sub _ _ _ _ _) (IHgamma _ _ _ _)) (incl_tran (perm_in nat_eq_dec perm_head) (fun o IN => _))).
+destruct IN as [EQ | IN].
+subst.
+apply (or_introl eq_refl).
+apply IN.
+Qed.
+
+Lemma ptree_bnd_l_inv_bot :
+    forall (phi : formula) (lambda kappa : ovar) (S : subst_ind),
+        ptree_bnd_l_inv bot phi lambda kappa S = bot.
+Proof.
+intros phi lambda kappa S.
+unfold ptree_bnd_l_inv, ptree_bnd_l_inv_fit.
+case (nat_eqb);
+reflexivity.
+Qed.
+
+(*
+Lemma ptree_bnd_l_inv_leaves :
+    forall (P : ptree) (A : formula) (v : ivar),
+        struct_valid P ->
+            forall (S : subst_ind),
+                (length (ptree_left P) = length S) ->
+                    In ((loop_head (ptree_constraint P) (ptree_left P) (ptree_right P) (ptree_deg P) bot), bot) (leaves P) ->
+                        In ((loop_head (ptree_constraint P) (batch_sub (ptree_left P) (univ v A) A S) (ptree_right P) (ptree_deg P) bot), bot) (leaves (ptree_bnd_l_inv P A v S)).
+Proof.
+intros P A v.
+induction P;
+try intros PSV S EQ INPL;
+unfold ptree_bnd_l_inv;
+unfold bnd_left_inv_batch, batch_sub.
+
+1-3 : destruct PSV.
+5-11 : destruct PSV as [[[[[PSV [PG_app PD_app]] PG] PD] POC] PDeg].
+12 : destruct PSV as [[[[[[[PSV [PG_app PD_app]] PG] PD] KNING] KNIND] [KIN POC]] PDeg].
+13-14 : destruct PSV as [[[[[PSV [PG_app PD_app]] PG] PD] POC] PDeg].
+15 : destruct PSV as [[[[[[PSV [PG_app PD_app]] PG] PD] POC] POC_rel] PDeg].
+16 : destruct PSV as [[[[[[PSV [PG_app PD_app]] PG] PD] [NEW [KIN POC]]] [NING NIND]] PDeg].
+17 : destruct PSV as [[[[[[[[[[P1SV P2SV] [PG_app PD_app]] P1G] P1D] P1OC] P2G] P2D] P2OC] PDeg1] PDeg2].
+18 : destruct PSV as [[[[[PSV [PG_app PD_app]] PG] PD] POC] PDeg].
+19 : destruct PSV as [[[[[[[[[[P1SV P2SV] [PG_app PD_app]] P1G] P1D] P1OC] P2G] P2D] P2OC] PDeg1] PDeg2].
+4 : destruct PSV as [[PSV [PG_app PD_app]] [PBot | [[[[[PRec PG] PD] POC] PDeg] PLoop]]].
+
+1-3 : inversion INPL as [].
+
+1 : { subst.
+      unfold ptree_constraint, ptree_left, ptree_right, ptree_deg in *.
+      rewrite EQ, nat_eqb_refl.
+      unfold ptree_bnd_l_inv_fit, leaves.
+      rewrite batch_sub_fit_true.
+      apply (or_introl eq_refl).
+      rewrite EQ.
+      apply nat_eqb_refl. }
+
+1 : { inversion INPL as [INPL' | FAL];
+      try inversion FAL.
+      unfold ptree_constraint, ptree_left, ptree_right, ptree_deg in INPL';
+      fold ptree_constraint ptree_left ptree_right ptree_deg in *.
+      inversion INPL' as [[EQ1 EQ2]].
+      subst.
+      contradiction PRec. }
+
+
+
+all : subst;
+      try rewrite EQ, nat_eqb_refl.
+
+      case nat_eqb eqn:EQ;
+      try apply INPL.
+      unfold ptree_bnd_l_inv_fit;
+      fold ptree_bnd_l_inv_fit;
+      unfold ptree_left in EQ;
+      fold ptree_left in EQ.
+
+2,4,5 : destruct S as [ | b S];
+        inversion EQ;
+        reflexivity.
+
+- destruct S as [ | b1 [ | b2 S]].
+  inversion EQ.
+  inversion EQ.
+  reflexivity.
+
+- destruct S as [ | b S].
+  inversion EQ.
+  case (nat_eqb v0 v && form_eqb phi A).
+  case b.
+  2,3 : reflexivity.
+  unfold ptree_deg at 2.
+  rewrite ptree_bnd_l_inv_fit_true.
+  apply (IHP PSV).
+  rewrite PG.
+  apply EQ.
+Qed.
+*)
+
+
+Lemma ptree_bnd_l_inv_height_aux :
+    forall (n : nat) (P : ptree) (A : formula) (lambda kappa : ovar),
+        ptree_height P <= n ->
+            forall (S : subst_ind),
+                ptree_height (ptree_bnd_l_inv_fit P A lambda kappa S) <= n.
+Proof.
+induction n;
+intros P A lambda kappa LT S.
+destruct P;
+inversion LT.
+destruct P;
+apply le_S_n in LT;
+unfold ptree_bnd_l_inv_fit;
+fold ptree_bnd_l_inv_fit;
+unfold ptree_height;
+fold ptree_height.
+
+4,8,11,13 : destruct S as [ | b S].
+
+9 : case (nat_eqb lambda0 lambda) eqn:EQL.
+9 : case (nat_eqb kappa0 kappa) eqn:EQK.
+9 : case (form_eqb phi A) eqn:EQF.
+9 : destruct b.
+
+all : unfold ptree_height in *;
+      fold ptree_height in *;
+      try apply le_n_S;
+      try rewrite EQL';
+      try apply (IHn _ _ _ _ LT);
+      try lia.
+
+- apply le_S, IHn, LT.
+
+- assert ((ptree_height P1) <= n /\ (ptree_height P2) <= n) as [LT1 LT2]. split; lia.
+  pose proof (IHn _ A lambda kappa LT1 (false :: S)) as LT3.
+  pose proof (IHn _ A lambda kappa LT2 S) as LT4.
+  lia.
+
+- assert ((ptree_height P1) <= n /\ (ptree_height P2) <= n) as [LT1 LT2]. split; lia.
+  pose proof (IHn _ A lambda kappa LT1 S) as LT3.
+  pose proof (IHn _ A lambda kappa LT2 (false :: S)) as LT4.
+  lia.
+Qed.
+
+(*
+Lemma ptree_bnd_l_inv_height :
+    forall (P : ptree) (A : formula) (S : subst_ind),
+        ptree_height (ptree_bnd_l_inv_fit P A S (ptree_height P)) <= (ptree_height P).
+Proof. intros P A S. apply (ptree_bnd_l_inv_height_aux _ _ _ (le_n _)). Qed.
+*)
+
+(*
+Lemma ptree_bnd_l_inv_fit_extra :
+    forall (d1 d2 : nat) (P : ptree) (A : formula) (S : subst_ind),
+        (ptree_height P) <= d1 ->
+            (ptree_height P) <= d2 ->
+                ptree_bnd_l_inv_fit P A S d1 = ptree_bnd_l_inv_fit P A S d2.
+Proof.
+induction d1;
+intros d2 P A S LT1 LT2.
+destruct P;
+inversion LT1.
+destruct d2.
+destruct P;
+inversion LT2.
+destruct P;
+apply le_S_n in LT1;
+apply le_S_n in LT2;
+unfold ptree_height in *;
+fold ptree_height in *;
+unfold ptree_bnd_l_inv_fit;
+fold ptree_bnd_l_inv_fit.
+
+6,7,12,15,17,19 : destruct S as [ | b S].
+
+5 : destruct S as [ | b1 [ | b2 S]].
+
+15 : destruct b.
+15 : case (form_eqb phi A) eqn:EQF.
+
+21,31 : assert (ptree_height P1 <= d1 /\ ptree_height P2 <= d1 /\ (ptree_height P1) <= d2 /\ (ptree_height P2) <= d2) as [LT3 [LT4 [LT5 LT6]]]; repeat split; try lia.
+
+all : try rewrite (IHd1 _ _ _ _ LT1 LT2);
+      try rewrite (IHd1 _ _ _ _ LT3 LT5);
+      try rewrite (IHd1 _ _ _ _ LT4 LT6);
+      try rewrite (IHd1 _ _ _ _ LT3);
+      try rewrite (IHd1 _ _ _ _ LT4);
+      try reflexivity.
+
+1 : pose proof (ptree_bnd_l_inv_height P (shift_substitution A (Datatypes.S v1) v2) (false :: b2 :: (repeat false (@length bool S)))) as LT3.
+    rewrite <- (IHd1 _ _ _ _ LT1 (le_n _)) in LT3.
+    rewrite (IHd1 _ _ _ _ LT1 LT2) in LT3.
+    rewrite (IHd1 _ _ _ _ (PeanoNat.Nat.le_trans _ _ _ LT3 LT1) (PeanoNat.Nat.le_trans _ _ _ LT3 LT2)).
+    reflexivity.
+Qed.
+*)
+
+Lemma ptree_bnd_l_inv_struct_aux :
+    forall (P : ptree) (A : formula) (lambda kappa : ovar),
+        struct_valid P ->
+            (OC_rel (ptree_constraint P) lambda kappa = true) ->
+                forall (S : subst_ind),
+                    struct_valid (ptree_bnd_l_inv P A lambda kappa S).
+Proof.
+intros P A lambda kappa.
+induction P;
+intros PSV REL S;
+unfold ptree_bnd_l_inv;
+case nat_eqb eqn:EQ;
+try apply PSV;
+unfold ptree_bnd_l_inv_fit;
+fold ptree_bnd_l_inv_fit.
+
+11 :  destruct S as [ | b S];
+      try apply PSV.
+
+6 :  destruct S as [ | b S];
+      try apply PSV.
+
+2 :  destruct S as [ | b S];
+      try apply PSV.
+
+9 : destruct S as [ | b S];
+    try apply PSV.
+
+1 : destruct PSV as [[PSV [PG_app PD_app]] [PBot | [[[[PRec PG] PD] POC] PDeg]]].
+3-8 : destruct PSV as [[[[[PSV [PG_app PD_app]] PG] PD] POC] PDeg].
+9 : destruct PSV as [[[[[[[PSV [PG_app PD_app]] PG] PD] KNING] KNIND] [KIN POC]] PDeg].
+10 : destruct PSV as [[[[[[PSV [PG_app PD_app]] PG] PD] POC] POC_rel] PDeg].
+11 : destruct PSV as [[[[[[PSV [PG_app PD_app]] PG] PD] POC] [NING NIND]] PDeg].
+12 : destruct PSV as [[[[[[[[[[P1SV P2SV] [PG_app PD_app]] P1G] P1D] P1OC] P2G] P2D] P2OC] PDeg1] PDeg2].
+13 : destruct PSV as [[[[[PSV [PG_app PD_app]] PG] PD] POC] PDeg].
+14 : destruct PSV as [[[[[[[[[[P1SV P2SV] [PG_app PD_app]] P1G] P1D] P1OC] P2G] P2D] P2OC] PDeg1] PDeg2].
+
+all : subst.
+
+10 :  case (nat_eqb lambda0 lambda) eqn:EQL;
+      try apply nat_eqb_eq in EQL;
+      subst.
+10 :  case (nat_eqb kappa0 kappa) eqn:EQK;
+      try apply nat_eqb_eq in EQK;
+      subst.
+10 :  case (form_eqb phi A) eqn:EQF;
+      try apply form_eqb_eq in EQF;
+      subst.
+10 : destruct b.
+
+2 : { rewrite ptree_bnd_l_inv_fit_true.
+      2 : apply EQ.
+      enough (struct_valid (loop_head (ptree_constraint P) (bnd_left_inv_batch (ptree_left P) A lambda kappa S) (ptree_right P) (ptree_deg P) (ptree_bnd_l_inv P A lambda kappa S))) as PSV'.
+      destruct P;
+      try apply PSV';
+      contradiction (PRec eq_refl).
+      repeat split.
+      - apply (IHP PSV REL).
+      - unfold ptree_left at 1.
+        unfold ptree_left at 1 in PG_app.
+        unfold ptree_constraint at 1 in REL.
+        apply (ptree_bnd_l_inv_vars _ _ _ _ _ _ REL PG_app).
+      - apply PD_app.
+      - destruct (ptree_eq_dec (ptree_bnd_l_inv P A lambda kappa S) bot) as [EQ' | NE].
+        apply (inl EQ').
+        right.
+        repeat split;
+        try apply EQ;
+        try rewrite ptree_bnd_l_inv_constraint;
+        try apply ptree_bnd_l_inv_deg;
+        try rewrite ptree_bnd_l_inv_left;
+        try rewrite ptree_bnd_l_inv_right;
+        try assumption;
+        try reflexivity. }
+
+1 : { repeat split.
+      - apply (ptree_bnd_l_inv_vars _ _ _ _ _ _ REL PG_app).
+      - apply PD_app.
+      - apply (inl eq_refl). }
+
+(*
+19 : rewrite (ptree_bnd_l_inv_fit_extra _ _ _ _ _ (PeanoNat.Nat.le_max_l _ _) (le_n _)), (ptree_bnd_l_inv_fit_extra _ _ _ _ _ (PeanoNat.Nat.le_max_r _ _) (le_n _)).
+
+17 : rewrite (ptree_bnd_l_inv_fit_extra _ _ _ _ _ (PeanoNat.Nat.le_max_l _ _) (le_n _)), (ptree_bnd_l_inv_fit_extra _ _ _ _ _ (PeanoNat.Nat.le_max_r _ _) (le_n _)).
+*)
+
+(*
+1 : { rewrite (ptree_bnd_l_inv_fit_extra _ _ _ _ _ (ptree_bnd_l_inv_height _ _ _) (le_n _)).
+      rewrite !ptree_bnd_l_inv_fit_true.
+      3 : rewrite !ptree_bnd_l_inv_fit_true;
+          try rewrite (ptree_bnd_l_inv_left _ _ PSV);
+          unfold bnd_left_inv_batch;
+          try rewrite <- batch_sub_length;
+          try apply nat_eqb_eq.
+      all : try rewrite PG;
+            unfold length;
+            fold (@length formula) (@length bool);
+            try rewrite repeat_length;
+            try apply EQ.
+      repeat split.
+      1 : { refine (IHd _ _ (PeanoNat.Nat.le_trans _ _ _ _ LT) (IHd _ _ LT PSV _) _).
+            pose proof (ptree_bnd_l_inv_height P (shift_substitution A (Datatypes.S v1) v2) (false :: b2 :: (repeat false (length S)))) as LT'.
+            rewrite !ptree_bnd_l_inv_fit_true in LT'.
+            apply LT'.
+            rewrite PG.
+            unfold length in *;
+            fold (@length formula) (@length bool) in *.
+            rewrite repeat_length.
+            apply EQ. }
+      1 : rewrite ptree_bnd_l_inv_vars;
+          unfold bnd_left_inv_batch;
+          apply PG_app.
+      1 : apply PD_app.
+      all : try rewrite !ptree_bnd_l_inv_left;
+            try rewrite !ptree_bnd_l_inv_right;
+            try rewrite !ptree_bnd_l_inv_constraint;
+            try rewrite !ptree_bnd_l_inv_deg;
+            try reflexivity;
+            try apply PSV;
+            try apply (IHd _ _ LT PSV).
+      unfold bnd_left_inv_batch.
+      unfold batch_sub at 1.
+      unfold ptree_left in EQ.
+      rewrite PG, <- batch_sub_length.
+      unfold batch_sub.
+      all : unfold length in *;
+            fold (@length bool) (@length formula) in *;
+            try rewrite repeat_length.
+      2 : apply (nat_eqb_eq _ _ EQ).
+      rewrite EQ.
+      unfold nat_eqb in EQ;
+      fold nat_eqb in EQ.
+      rewrite EQ.
+      unfold batch_sub_fit;
+      fold batch_sub_fit.
+      rewrite batch_sub_false.
+      unfold formula_sub, form_eqb;
+      fold form_eqb.
+      case (form_eqb (shift_substitution phi v1 v2) (univ (shift_substitution A (Datatypes.S v1) v2))) eqn:EQF.
+      destruct b2.
+      - assert (form_eqb (shift_substitution phi v1 v2) (shift_substitution (univ A) v1 v2) = true) as EQF'. apply EQF.
+        case form_eqb.
+        unfold bnd_left_inv_formula, formula_sub.
+        admit.
+        admit.
+      - case form_eqb;
+        unfold bnd_left_inv_formula;
+        rewrite formula_sub_false;
+        reflexivity.
+      - assert (form_eqb (shift_substitution phi v1 v2) (shift_substitution (univ A) v1 v2) = false) as EQF'. apply EQF.
+        case form_eqb;
+        unfold bnd_left_inv_formula, formula_sub;
+        rewrite (shift_subst_neb_form_neb _ _ _ _ EQF');
+        reflexivity. }
+
+18 : assert ((ptree_height P1) <= d /\ (ptree_height P2) <= d) as [LT1 LT2].
+18 : split; lia.
+
+16 : assert ((ptree_height P1) <= d /\ (ptree_height P2) <= d) as [LT1 LT2].
+16 : split; lia.
+*)
+
+7 : { rewrite ptree_bnd_l_inv_fit_true;
+      try rewrite PG;
+      try rewrite P1G;
+      try rewrite P2G;
+      try apply EQ;
+      unfold ptree_left at 1 in EQ;
+      try rewrite bury_length, <- (@bury_unbury _ S n), bury_length in EQ;
+      try apply EQ;
+      repeat split;
+      try rewrite ptree_bnd_l_inv_constraint;
+      try apply ptree_bnd_l_inv_deg;
+      try rewrite ptree_bnd_l_inv_left;
+      try rewrite PG;
+      try rewrite P1G;
+      try rewrite P2G;
+      unfold flat_map;
+      fold (flat_map vars_in);
+      unfold bnd_left_inv_batch;
+      try rewrite batch_sub_false_head;
+      try rewrite ptree_bnd_l_inv_right;
+      try assumption;
+      try apply (IHP PSV REL);
+      try apply (IHP1 P1SV REL);
+      try rewrite <- P2OC in REL;
+      try apply (IHP2 P2SV REL);
+      try reflexivity.
+      2 : unfold ptree_left at 1;
+          apply (ptree_bnd_l_inv_vars _ _ _ _ _ _ REL PG_app).
+      apply IHP.
+      apply PSV.
+      rewrite POC.
+      unfold restriction, OC_rel at 1, projT2, projT1.
+      unfold ptree_constraint in REL.
+      rewrite REL, andb_true_l.
+       }
+
+all : repeat rewrite ptree_bnd_l_inv_fit_true;
+      try rewrite PG;
+      try rewrite P1G;
+      try rewrite P2G;
+      try apply EQ;
+      unfold ptree_left at 1 in EQ;
+      try rewrite bury_length, <- (@bury_unbury _ S n), bury_length in EQ;
+      try apply EQ;
+      repeat split;
+      try rewrite ptree_bnd_l_inv_constraint;
+      try apply ptree_bnd_l_inv_deg;
+      try rewrite ptree_bnd_l_inv_left;
+      try rewrite PG;
+      try rewrite P1G;
+      try rewrite P2G;
+      unfold flat_map;
+      fold (flat_map vars_in);
+      unfold bnd_left_inv_batch;
+      try rewrite batch_sub_false_head;
+      try rewrite ptree_bnd_l_inv_right;
+      try assumption;
+      try apply (IHP PSV REL);
+      try apply (IHP1 P1SV REL);
+      try rewrite <- P2OC in REL;
+      try apply (IHP2 P2SV REL);
+      try reflexivity.
+
+14 :  { intros FAL.
+        apply NING.
+        unfold ptree_constraint at 1 in REL.
+        unfold ptree_left at 1 in PG_app.
+        pose proof (ptree_bnd_l_inv_vars_sub _ _ _ _ _ _ FAL) as [FAL1 | FAL2].
+        subst.
+        destruct POC as [NEW].
+        contradict (NEW (proj1 (OC_null _ _ _ REL))).
+        apply FAL2. }
+
+12 :  { apply (IHP PSV).
+        destruct POC as [NEW [KIN POC]].
+        rewrite POC.
+        unfold OC_rel, add_fresh_child, projT2, projT1.
+        unfold ptree_constraint at 1 in REL.
+        rewrite REL.
+        reflexivity. }
+
+(*
+10 :  { intros FAL.
+        apply KNING.
+        unfold ptree_constraint at 1 in REL.
+        unfold ptree_left at 1 in PG_app.
+        pose proof (struct_OC_app _ PSV) as [P'G_app P'D_app].
+        rewrite POC in *.
+        pose proof (ptree_bnd_l_inv_vars_sub _ _ _ _ _ _ FAL) as [FAL1 | FAL2].
+        subst.
+
+        admit.
+        apply FAL2. }
+
+8 : { apply (IHP PSV).
+      rewrite POC.
+      unfold OC_rel, restriction, projT2, projT1.
+      unfold ptree_constraint at 1 in REL.
+      rewrite REL.
+      case (in_dec nat_eq_dec lambda (children OC kappa0)) as [FAL | _].
+      unfold children in FAL.
+      apply filter_In in FAL as [FAL1 FAL2].
+      admit.
+      case (in_dec nat_eq_dec kappa (children OC kappa0)) as [FAL | _].
+      admit.
+      reflexivity. }*)
+
+2 : try rewrite <- batch_sub_fit_true;
+    unfold batch_sub_fit;
+    fold batch_sub_fit;
+    try rewrite batch_sub_fit_true;
+    try reflexivity;
+    try apply EQ.
+
+all : unfold ptree_left at 1;
+      try apply (ptree_bnd_l_inv_vars _ _ _ _ _ _ REL PG_app).
+
+2 : { intros o IN.
+      rewrite flat_map_bury_incl in IN.
+      pose proof (ptree_bnd_l_inv_vars (ptree_left P) A lambda kappa (unbury S n) (ptree_constraint P) REL (fun o' IN' => PG_app o' (proj2 (flat_map_bury_incl o') IN'))) as SUB.
+      apply SUB, IN. }
+
+1 : pose proof (ptree_bnd_l_inv_vars (phi :: gamma) A lambda kappa (b :: S) (ptree_constraint P) REL PG_app) as SUB.
+2 : pose proof (ptree_bnd_l_inv_vars (phi :: (ptree_left P)) A lambda kappa (b :: S) (ptree_constraint P) REL PG_app) as SUB.
+3-6 : pose proof (ptree_bnd_l_inv_vars _ A _ _ (false :: S) _ REL PG_app) as SUB.
+7 : fold (ptree_constraint (@imp_l (ptree_constraint P1) (ptree_left P2) (ptree_right P1) phi psi (ptree_deg P1) (ptree_deg P2) P1 P2)) in PG_app;
+    rewrite <- P2OC in PG_app;
+    pose proof (ptree_bnd_l_inv_vars _ A _ _ (false :: S) _ REL PG_app) as SUB;
+    unfold ptree_constraint at 1 in SUB;
+    rewrite P2OC in SUB.
+8 : fold (ptree_constraint (@cut (ptree_constraint P1) (ptree_left P1) (ptree_right P2) phi (ptree_deg P1) (ptree_deg P2) P1 P2)) in PG_app;
+    rewrite <- P2OC in PG_app;
+    pose proof (ptree_bnd_l_inv_vars _ A _ _ S _ REL PG_app) as SUB;
+    unfold ptree_constraint at 1 in SUB;
+    rewrite P2OC in SUB.
+
+
+1-6 : unfold ptree_left, bnd_left_inv_batch, batch_sub, batch_sub_fit, length, nat_eqb in SUB;
+      fold (ptree_left P) batch_sub_fit (@length bool) (@length formula) nat_eqb in SUB;
+      unfold length, nat_eqb in EQ;
+      fold (@length bool) (@length formula) nat_eqb in EQ;
+      try rewrite EQ in SUB;
+      rewrite batch_sub_fit_true in SUB;
+      try rewrite formula_sub_false in SUB;
+      try apply SUB;
+      try apply EQ.
+
+1,2 : unfold ptree_left, bnd_left_inv_batch, batch_sub, batch_sub_fit, length, nat_eqb in SUB;
+    fold (ptree_left P1) (ptree_left P2) batch_sub_fit (@length bool) (@length formula) nat_eqb in SUB;
+    unfold length, nat_eqb in EQ;
+    fold (@length bool) (@length formula) nat_eqb in EQ;
+    try rewrite EQ in SUB;
+    rewrite batch_sub_fit_true in SUB;
+    try rewrite formula_sub_false in SUB;
+    try apply SUB;
+    try apply EQ.
+Admitted.
